src/Narcissus/Formats.v
@@ -1,4 +1,10 @@
 Require Export
-        Fiat.Narcissus.Formats.WordOpt
+        Fiat.Narcissus.Formats.FixListOpt
+        Fiat.Narcissus.Formats.Bool
         Fiat.Narcissus.Formats.NatOpt
-        Fiat.Narcissus.Formats.FixListOpt.
+        Fiat.Narcissus.Formats.Vector
+        Fiat.Narcissus.Formats.EnumOpt
+        Fiat.Narcissus.Formats.SumTypeOpt
+        Fiat.Narcissus.Formats.IPChecksum
+        Fiat.Narcissus.Formats.WordOpt
+        Fiat.Narcissus.Formats.NatOpt.
